Add an extra assumption to minimal parse trees
Requiring that everything in the tree be in the valid list lets us
weaken the interface of the boolean parser, allowing the splitter to
only be complete for productions it will actually be called on.

src/Common.v
@@ -1196,3 +1196,28 @@ Definition option_bind {A} {B} (f : A -> option B) (x : option A)
        | None => None
        | Some a => f a
      end.
+
+Fixpoint ForallT {T} (P : T -> Type) (ls : list T) : Type
+  := match ls return Type with
+       | nil => True
+       | x::xs => (P x * ForallT P xs)%type
+     end.
+Fixpoint Forall_tails {T} (P : list T -> Type) (ls : list T) : Type
+  := match ls with
+       | nil => P nil
+       | x::xs => (P (x::xs) * Forall_tails P xs)%type
+     end.
+
+Fixpoint ForallT_all {T} {P : T -> Type} (p : forall t, P t) {ls}
+: ForallT P ls
+  := match ls with
+       | nil => I
+       | x::xs => (p _, @ForallT_all T P p xs)
+     end.
+
+Fixpoint Forall_tails_all {T} {P : list T -> Type} (p : forall t, P t) {ls}
+: Forall_tails P ls
+  := match ls with
+       | nil => p _
+       | x::xs => (p _, @Forall_tails_all T P p xs)
+     end.
